Challenge/Modexp/Submission/Proofs/Bytecode/UnrollPCs.lean
@@ -27,31 +27,31 @@ open YulEvmCompiler
   rw [Challenge.Modexp.Submission.Proofs.Bytecode.PCFast.instructionPC_eq_byteLength]
   rfl
 
-@[simp] theorem pc2414 : Artifact.submissionArtifact.instructionPC 1797 = 2376 := by
+@[simp] theorem pc2414 : Artifact.submissionArtifact.instructionPC 1590 = 2115 := by
   rw [Challenge.Modexp.Submission.Proofs.Bytecode.PCFast.instructionPC_eq_byteLength]
   rfl
 
-@[simp] theorem pc2415 : Artifact.submissionArtifact.instructionPC 1798 = 2377 := by
+@[simp] theorem pc2415 : Artifact.submissionArtifact.instructionPC 1591 = 2116 := by
   rw [Challenge.Modexp.Submission.Proofs.Bytecode.PCFast.instructionPC_eq_byteLength]
   rfl
 
-@[simp] theorem pc2416 : Artifact.submissionArtifact.instructionPC 1799 = 2379 := by
+@[simp] theorem pc2416 : Artifact.submissionArtifact.instructionPC 1592 = 2118 := by
   rw [Challenge.Modexp.Submission.Proofs.Bytecode.PCFast.instructionPC_eq_byteLength]
   rfl
 
-@[simp] theorem pc2417 : Artifact.submissionArtifact.instructionPC 1800 = 2380 := by
+@[simp] theorem pc2417 : Artifact.submissionArtifact.instructionPC 1593 = 2119 := by
   rw [Challenge.Modexp.Submission.Proofs.Bytecode.PCFast.instructionPC_eq_byteLength]
   rfl
 
-@[simp] theorem pc2554 : Artifact.submissionArtifact.instructionPC 1829 = 2417 := by
+@[simp] theorem pc2554 : Artifact.submissionArtifact.instructionPC 1622 = 2156 := by
   rw [Challenge.Modexp.Submission.Proofs.Bytecode.PCFast.instructionPC_eq_byteLength]
   rfl
 
-@[simp] theorem pc2555 : Artifact.submissionArtifact.instructionPC 1830 = 2418 := by
+@[simp] theorem pc2555 : Artifact.submissionArtifact.instructionPC 1623 = 2157 := by
   rw [Challenge.Modexp.Submission.Proofs.Bytecode.PCFast.instructionPC_eq_byteLength]
   rfl
 
-@[simp] theorem pc2556 : Artifact.submissionArtifact.instructionPC 1831 = 2420 := by
+@[simp] theorem pc2556 : Artifact.submissionArtifact.instructionPC 1624 = 2159 := by
   rw [Challenge.Modexp.Submission.Proofs.Bytecode.PCFast.instructionPC_eq_byteLength]
   rfl
 
